#P3.1
---
(a)  
$$y(t)=x_{1}(t),  \dot{y}=x_{2}(t),  \ddot{y}=\dot{x_{2}}(t)$$

(b)

$$M\ddot{y}(t)=-ky(t)-b\dot{y}(t)+F(t) $$

$$\ddot{y}(t)=-\frac{k}{M}y(t)-\frac{b}{M}\dot{y}(t)+\frac{1}{M}F(t) $$

$$\dot{x_{2}}(t)=-\frac{k}{M}x_{1}(t)-\frac{b}{M}x_{2}(t)+\frac{1}{M}F(t)  $$

$$\dot{x_{1}}(t)=x_{2}(t)  $$

(c)  
$$\dot{x}(t)=\begin{bmatrix}0 & 1 \\-\frac{k}{M} & -\frac{b}{M} \end{bmatrix}x(t)+\left(\begin{array}{c}0\\ \frac{1}{M}\end{array}\right)F(t)$$

$$y(t)=y(t)=\begin{bmatrix}1 & 0 \end{bmatrix}x_{1}(t)$$

#P3.3
---
Apply KCL  
$$i_{L}(t)+\frac{V_{0}}{R}=i_{c}(t)$$
$$i_{L}(t)+\frac{V_{0}}{R}=-C\frac{\text{d}V_{c}(t)}{\text{d}t}$$
$$C\frac{\text{d}V_{c}(t)}{\text{d}t}=-\frac{V_{2}-V_{c}(t)}{R}-i_{L}(t)$$
$$\frac{\text{d}v_{c}(t)}{\text{d}t}=-\frac{v_{2}-v_{c}(t)}{CR}-\frac{1}{C}i_{L}(t)$$
$$\dot{x_{2}}(t)=-\frac{1}{C}\dot{x_{1}}(t)-\frac{1}{RC}x_{2}(t)$$


Apply KVL
$$-V_{1}+L\frac{\text{d}i_{L}(t)}{\text{d}t}-V_{C}(t)+V_{2}(t)$$
$$\frac{\text{d}i_{L}(t)}{\text{d}t}=\frac{v_{1}(t)}{L}+\frac{v_{c}(t)}{L}-\frac{v_{2}(t)}{L}$$
$$\dot{x_{1}}(t)=\frac{1}{L}x_{2}(t)+\frac{1}{L}v_{1}(t)-\frac{1}{L}v_{2}(t)$$

therefore
$$\dot{x}(t)=\begin{bmatrix}0 & \frac{1}{L} \\-\frac{1}{C} & -\frac{1}{RC} \end{bmatrix}x(t)+\begin{bmatrix}\frac{1}{L} & -\frac{1}{L} \\0 & 0 \end{bmatrix}$$


#P3.5
---
$$T(s)=\frac{Y(s)}{R(s)}=\frac{s+2}{s^3+5s^2-23s+2}$$
$$Y(s)=(s+2)Z(s)$$
$$y(t)=\dot{z}(t)+2z(t)$$
$$y(t)=x_{2}(t)+x_{1}(t)$$
$$R(s)=(s^3+5s^2-23s+2)Z(s)$$
$$r(t)=\dddot{z}(t)+5\ddot{z}(t)-23\dot{z}(t)+2z(t)$$
$$\dot{x_{3}}(t)=-2x_{1}(t)+23x_{2}(t)-5x_{3}(t)+r(t)$$
$$\dot{x_{2}}(t)=x_{2}(t)$$
$$\dot{x_{2}}(t)=x_{3}(t)$$

$$\dot{x}(t)=\begin{bmatrix}0 & 1 & 0  \\0 & 0 & 1\\-2 & 23 & -5\end{bmatrix}x(t)+\begin{bmatrix}0 \\0\\1 \end{bmatrix}r(t)$$
$$y(t)=\begin{bmatrix}2 & 1 &0 \end{bmatrix}x(t)$$

#P3.12
---
(a)
$$Y(s)=(8s+40)Z(s)$$
$$y(t)=\dot{z}(t)+40z(t)=8x_{2}(t)+40x_{1}(t)$$
$$R(s)=(s^3+12s^2+44s+48)Z(s)$$
$$r(t)=\dddot{z}(t)+12\ddot{z}(t)+44\dot{z}(t)+48z(t)$$
$$\dot{x_{3}}(t)=-12x_{3}(t)-44x_{2}(t)-48x_{3}(t)+r(t)$$
$$\dot{x_{1}}(t)=x_{2}(t)$$
$$\dot{x_{2}}(t)=x_{3}(t)$$
$$\dot{x}(t)=\begin{bmatrix}0 & 1 & 0  \\0 & 0 & 1\\-48 & -44 & -12\end{bmatrix}x(t)+\begin{bmatrix}0 \\0\\1 \end{bmatrix}r(t)$$
$$y(t)=\begin{bmatrix}40 & 8  \end{bmatrix}x(t)$$

(b)
```
A = [0 1 0; 0 0 1; -48 -44 -12];
B = [0; 0; 1];
C = [40 8];
D = 0;
syms s
Phi = inv(s*eye(3)-A);
Phi_t = ilaplace(Phi)
```


#P3.17
---
```
A = [1 1 -1; 4 3 0; -2 1 10];
B = [0; 0; 4];
C = [1 0 0];
D = 0;
syms s
Phi = inv(s*eye(3)-A);
G = C * Phi * B + D;
pretty(G)
```









